amm exponentiation

code/bignum/Hacl.Bignum.Exponentiation.fst
@@ -16,9 +16,12 @@ module SM = Hacl.Spec.Bignum.Montgomery
 
 module BN = Hacl.Bignum
 module BM = Hacl.Bignum.Montgomery
+module AM = Hacl.Bignum.AlmostMontgomery
 module ME = Hacl.Bignum.MontExponentiation
+module AE = Hacl.Bignum.AlmostMontExponentiation
 
 module E = Hacl.Spec.Exponentiation.Lemmas
+module M = Hacl.Spec.Montgomery.Lemmas
 module SE = Hacl.Spec.Bignum.MontExponentiation
 module S = Hacl.Spec.Bignum.Exponentiation
 
@@ -40,13 +43,13 @@ let bn_check_mod_exp #t len n a bBits b =
 
 
 inline_for_extraction noextract
-val mk_bn_mod_exp_precomp:
+val mk_bn_mod_exp_precomp_mont:
     #t:limb_t
   -> k:BM.mont t
   -> bn_exp_mont: ME.bn_exp_mont_st t k.BM.bn.BN.len ->
   bn_mod_exp_precomp_st t k.BM.bn.BN.len
 
-let mk_bn_mod_exp_precomp #t k bn_exp_mont n mu r2 a bBits b res =
+let mk_bn_mod_exp_precomp_mont #t k bn_exp_mont n mu r2 a bBits b res =
   let h0 = ST.get () in
   [@inline_let] let len = k.BM.bn.BN.len in
   push_frame ();
@@ -66,17 +69,58 @@ let mk_bn_mod_exp_precomp #t k bn_exp_mont n mu r2 a bBits b res =
   pop_frame ()
 
 
+inline_for_extraction noextract
+val mk_bn_mod_exp_precomp_amont:
+    #t:limb_t
+  -> k:AM.almost_mont t
+  -> bn_exp_amont: AE.bn_exp_almost_mont_st t k.AM.bn.BN.len ->
+  bn_mod_exp_precomp_st t k.AM.bn.BN.len
+
+let mk_bn_mod_exp_precomp_amont #t k bn_exp_amont n mu r2 a bBits b res =
+  let h0 = ST.get () in
+  [@inline_let] let len = k.AM.bn.BN.len in
+  push_frame ();
+  BD.bn_eval_bound (as_seq h0 n) (v len);
+  let aM = create len (uint #t #SEC 0) in
+  AM.to n mu r2 a aM;
+  SM.bn_to_mont_lemma (as_seq h0 n) mu (as_seq h0 r2) (as_seq h0 a);
+  M.to_mont_lemma (bits t) (v len) (bn_v h0 n) (v mu) (bn_v h0 a);
+
+  let resM = create len (uint #t #SEC 0) in
+  bn_exp_amont n mu r2 aM bBits b resM;
+  AM.from n mu resM res;
+
+  let h1 = ST.get () in
+  SM.bn_from_mont_lemma (as_seq h0 n) mu (as_seq h1 resM);
+  BD.bn_eval_bound (as_seq h1 resM) (v len);
+  E.mod_exp_mont_ll_mod_lemma (bits t) (v len) (bn_v h0 n) (v mu) (bn_v h0 a) (bn_v h0 b) (bn_v h1 resM);
+  assert (bn_v h1 res == Lib.NatMod.pow_mod #(bn_v h0 n) (bn_v h0 a) (bn_v h0 b));
+  pop_frame ()
+
+
 let bn_mod_exp_bm_vartime_precomp #t k n mu r2 a bBits b res =
-  mk_bn_mod_exp_precomp #t k (ME.bn_exp_mont_bm_vartime #t k) n mu r2 a bBits b res
+  mk_bn_mod_exp_precomp_mont #t k (ME.bn_exp_mont_bm_vartime #t k) n mu r2 a bBits b res
 
 let bn_mod_exp_bm_consttime_precomp #t k n mu r2 a bBits b res =
-  mk_bn_mod_exp_precomp #t k (ME.bn_exp_mont_bm_consttime #t k) n mu r2 a bBits b res
+  mk_bn_mod_exp_precomp_mont #t k (ME.bn_exp_mont_bm_consttime #t k) n mu r2 a bBits b res
 
 let bn_mod_exp_fw_vartime_precomp #t k l n mu r2 a bBits b res =
-  mk_bn_mod_exp_precomp #t k (ME.bn_exp_mont_fw_vartime #t k l) n mu r2 a bBits b res
+  mk_bn_mod_exp_precomp_mont #t k (ME.bn_exp_mont_fw_vartime #t k l) n mu r2 a bBits b res
 
 let bn_mod_exp_fw_consttime_precomp #t k l n mu r2 a bBits b res =
-  mk_bn_mod_exp_precomp #t k (ME.bn_exp_mont_fw_consttime #t k l) n mu r2 a bBits b res
+  mk_bn_mod_exp_precomp_mont #t k (ME.bn_exp_mont_fw_consttime #t k l) n mu r2 a bBits b res
+
+let bn_mod_exp_amm_bm_vartime_precomp #t k n mu r2 a bBits b res =
+  mk_bn_mod_exp_precomp_amont #t k (AE.bn_exp_almost_mont_bm_vartime #t k) n mu r2 a bBits b res
+
+let bn_mod_exp_amm_bm_consttime_precomp #t k n mu r2 a bBits b res =
+  mk_bn_mod_exp_precomp_amont #t k (AE.bn_exp_almost_mont_bm_consttime #t k) n mu r2 a bBits b res
+
+let bn_mod_exp_amm_fw_vartime_precomp #t k l n mu r2 a bBits b res =
+  mk_bn_mod_exp_precomp_amont #t k (AE.bn_exp_almost_mont_fw_vartime #t k l) n mu r2 a bBits b res
+
+let bn_mod_exp_amm_fw_consttime_precomp #t k l n mu r2 a bBits b res =
+  mk_bn_mod_exp_precomp_amont #t k (AE.bn_exp_almost_mont_fw_consttime #t k l) n mu r2 a bBits b res
 
 
 let bn_mod_exp_consttime_precomp #t len bn_mod_exp_bm_consttime_precomp bn_mod_exp_fw_consttime_precomp n mu r2 a bBits b res =
@@ -93,7 +137,7 @@ let bn_mod_exp_vartime_precomp #t len bn_mod_exp_bm_vartime_precomp bn_mod_exp_f
     bn_mod_exp_fw_vartime_precomp n mu r2 a bBits b res
 
 
-let mk_bn_mod_exp_precompr2 #t k bn_mod_exp_precomp n r2 a bBits b res =
+let mk_bn_mod_exp_precompr2 #t len bn_mod_exp_precomp n r2 a bBits b res =
   let h0 = ST.get () in
   let mu = BM.mod_inv_limb n.(0ul) in // n * mu = 1 (mod (pow2 64))
   Hacl.Spec.Bignum.ModInvLimb.bn_mod_inv_limb_lemma (as_seq h0 n);
@@ -115,16 +159,16 @@ let bn_check_mod_exp_u32 (len:BN.meta_len U32) : bn_check_mod_exp_st U32 len =
   bn_check_mod_exp len
 let bn_mod_exp_vartime_precomp_u32 (len:BN.meta_len U32) : bn_mod_exp_precomp_st U32 len =
   [@inline_let]
-  let km = BM.mk_runtime_mont len in
+  let km = AM.mk_runtime_almost_mont len in
   bn_mod_exp_vartime_precomp len
-    (bn_mod_exp_bm_vartime_precomp km)
-    (bn_mod_exp_fw_vartime_precomp km 4ul)
+    (bn_mod_exp_amm_bm_vartime_precomp km)
+    (bn_mod_exp_amm_fw_vartime_precomp km 4ul)
 let bn_mod_exp_consttime_precomp_u32 (len:BN.meta_len U32) : bn_mod_exp_precomp_st U32 len =
   [@inline_let]
-  let km = BM.mk_runtime_mont len in
+  let km = AM.mk_runtime_almost_mont len in
   bn_mod_exp_consttime_precomp len
-    (bn_mod_exp_bm_consttime_precomp km)
-    (bn_mod_exp_fw_consttime_precomp km 4ul)
+    (bn_mod_exp_amm_bm_consttime_precomp km)
+    (bn_mod_exp_amm_fw_consttime_precomp km 4ul)
 let bn_mod_exp_vartime_u32 (len:BN.meta_len U32) : bn_mod_exp_st U32 len =
   mk_bn_mod_exp len (BM.bn_precomp_r2_mod_n_u32 len) (bn_mod_exp_vartime_precomp_u32 len)
 let bn_mod_exp_consttime_u32 (len:BN.meta_len U32) : bn_mod_exp_st U32 len =
@@ -148,16 +192,16 @@ let bn_check_mod_exp_u64 (len:BN.meta_len U64) : bn_check_mod_exp_st U64 len =
   bn_check_mod_exp len
 let bn_mod_exp_vartime_precomp_u64 (len:BN.meta_len U64) : bn_mod_exp_precomp_st U64 len =
   [@inline_let]
-  let km = BM.mk_runtime_mont len in
+  let km = AM.mk_runtime_almost_mont len in
   bn_mod_exp_vartime_precomp len
-    (bn_mod_exp_bm_vartime_precomp km)
-    (bn_mod_exp_fw_vartime_precomp km 4ul)
+    (bn_mod_exp_amm_bm_vartime_precomp km)
+    (bn_mod_exp_amm_fw_vartime_precomp km 4ul)
 let bn_mod_exp_consttime_precomp_u64 (len:BN.meta_len U64) : bn_mod_exp_precomp_st U64 len =
   [@inline_let]
-  let km = BM.mk_runtime_mont len in
+  let km = AM.mk_runtime_almost_mont len in
   bn_mod_exp_consttime_precomp len
-    (bn_mod_exp_bm_consttime_precomp km)
-    (bn_mod_exp_fw_consttime_precomp km 4ul)
+    (bn_mod_exp_amm_bm_consttime_precomp km)
+    (bn_mod_exp_amm_fw_consttime_precomp km 4ul)
 let bn_mod_exp_vartime_u64 (len:BN.meta_len U64) : bn_mod_exp_st U64 len =
   mk_bn_mod_exp len (BM.bn_precomp_r2_mod_n_u64 len) (bn_mod_exp_vartime_precomp_u64 len)
 let bn_mod_exp_consttime_u64 (len:BN.meta_len U64) : bn_mod_exp_st U64 len =
