code/bignum/Hacl.Bignum.AlmostMontExponentiation.fst
@@ -1,0 +1,269 @@
+module Hacl.Bignum.AlmostMontExponentiation
+
+open FStar.HyperStack
+open FStar.HyperStack.ST
+open FStar.Mul
+
+open Lib.IntTypes
+open Lib.Buffer
+
+open Hacl.Bignum.Definitions
+
+module ST = FStar.HyperStack.ST
+module LSeq = Lib.Sequence
+
+module BD = Hacl.Spec.Bignum.Definitions
+module SN = Hacl.Spec.Bignum
+module SM = Hacl.Spec.Bignum.Montgomery
+module SA = Hacl.Spec.Bignum.AlmostMontgomery
+
+module BN = Hacl.Bignum
+module BM = Hacl.Bignum.Montgomery
+module AM = Hacl.Bignum.AlmostMontgomery
+
+module LE = Lib.Exponentiation
+module BE = Hacl.Impl.Exponentiation
+module E = Hacl.Spec.Exponentiation.Lemmas
+module A = Hacl.Spec.AlmostMontgomery.Lemmas
+module ME = Hacl.Spec.Bignum.MontExponentiation
+
+module S = Hacl.Spec.Bignum.AlmostMontExponentiation
+
+#reset-options "--z3rlimit 50 --fuel 0 --ifuel 0"
+
+inline_for_extraction noextract
+let a_spec (#t:limb_t) (#len:SN.bn_len t) (n:BD.lbignum t len{0 < BD.bn_v n}) =
+  Lib.NatMod.nat_mod (BD.bn_v n)
+
+inline_for_extraction noextract
+let linv (#t:limb_t) (#len:SN.bn_len t) (n:BD.lbignum t len) (a:BD.lbignum t len) : Type0 =
+  BD.bn_v a < pow2 (bits t * len)
+
+inline_for_extraction noextract
+let refl (#t:limb_t) (#len:SN.bn_len t) (n:BD.lbignum t len{0 < BD.bn_v n}) (a:BD.lbignum t len{linv n a}) : a_spec n =
+  BD.bn_v a % BD.bn_v n
+
+inline_for_extraction noextract
+let linv_ctx (#t:limb_t) (#len:SN.bn_len t) (n:BD.lbignum t len) (a:BD.lbignum t len) : Type0 =
+  n == a
+
+
+inline_for_extraction noextract
+let mk_to_nat_mont_ll_comm_monoid
+  (t:limb_t)
+  (len:BN.meta_len t)
+  (n:BD.lbignum t (v len))
+  (mu:limb t{SM.bn_mont_pre n mu})
+  : BE.to_comm_monoid t len len =
+{
+  BE.a_spec = a_spec n;
+  BE.comm_monoid = E.mk_nat_mont_ll_comm_monoid (bits t) (v len) (BD.bn_v n) (v mu);
+  BE.linv_ctx = linv_ctx n;
+  BE.linv = linv n;
+  BE.refl = refl n;
+}
+
+
+inline_for_extraction noextract
+let bn_almost_mont_one_st (t:limb_t) (len:BN.meta_len t) =
+    n:lbignum t len
+  -> mu:limb t
+  -> r2:lbignum t len
+  -> oneM:lbignum t len ->
+  Stack unit
+  (requires fun h ->
+    live h n /\ live h r2 /\ live h oneM /\
+    disjoint n r2 /\ disjoint n oneM /\ disjoint r2 oneM /\
+
+    SM.bn_mont_pre (as_seq h n) mu /\
+    bn_v h r2 == pow2 (2 * bits t * v len) % bn_v h n)
+  (ensures  fun h0 _ h1 -> modifies (loc oneM) h0 h1 /\
+    bn_v h1 oneM % bn_v h0 n == E.mont_one_ll (bits t) (v len) (bn_v h0 n) (v mu) /\
+    bn_v h1 oneM < pow2 (bits t * v len))
+
+
+inline_for_extraction noextract
+val bn_almost_mont_one: #t:limb_t -> k:AM.almost_mont t -> bn_almost_mont_one_st t k.AM.bn.BN.len
+let bn_almost_mont_one #t k n mu r2 oneM =
+  let h0 = ST.get () in
+  BM.bn_mont_one k.AM.bn.BN.len k.AM.from n mu r2 oneM;
+  let h1 = ST.get () in
+  SM.bn_mont_one_lemma (as_seq h0 n) mu (as_seq h0 r2);
+  Math.Lemmas.small_mod (bn_v h1 oneM) (bn_v h0 n);
+  BD.bn_eval_bound (as_seq h1 oneM) (v k.AM.bn.BN.len)
+
+
+inline_for_extraction noextract
+val bn_almost_mont_mul:
+    #t:limb_t
+  -> k:AM.almost_mont t
+  -> n:Ghost.erased (BD.lbignum t (v k.AM.bn.BN.len))
+  -> mu:limb t{SM.bn_mont_pre n mu} ->
+  BE.lmul_st t k.AM.bn.BN.len k.AM.bn.BN.len (mk_to_nat_mont_ll_comm_monoid t k.AM.bn.BN.len n mu)
+
+let bn_almost_mont_mul #t k n mu ctx aM bM resM =
+  let h0 = ST.get () in
+  SA.bn_almost_mont_mul_lemma n mu (as_seq h0 aM) (as_seq h0 bM);
+  A.almost_mont_mul_is_mont_mul_lemma (bits t) (v k.AM.bn.BN.len) (BD.bn_v n) (v mu) (bn_v h0 aM) (bn_v h0 bM);
+  k.AM.mul ctx mu aM bM resM
+
+
+inline_for_extraction noextract
+val bn_almost_mont_sqr:
+    #t:limb_t
+  -> k:AM.almost_mont t
+  -> n:Ghost.erased (BD.lbignum t (v k.AM.bn.BN.len))
+  -> mu:limb t{SM.bn_mont_pre n mu} ->
+  BE.lsqr_st t k.AM.bn.BN.len k.AM.bn.BN.len (mk_to_nat_mont_ll_comm_monoid t k.AM.bn.BN.len n mu)
+
+let bn_almost_mont_sqr #t k n mu ctx aM resM =
+  let h0 = ST.get () in
+  SA.bn_almost_mont_sqr_lemma n mu (as_seq h0 aM);
+  SA.bn_almost_mont_mul_lemma n mu (as_seq h0 aM) (as_seq h0 aM);
+  A.almost_mont_mul_is_mont_mul_lemma (bits t) (v k.AM.bn.BN.len) (BD.bn_v n) (v mu) (bn_v h0 aM) (bn_v h0 aM);
+  k.AM.sqr ctx mu aM resM
+
+
+inline_for_extraction noextract
+let mk_bn_almost_mont_concrete_ops
+  (t:limb_t)
+  (k:AM.almost_mont t)
+  (n:Ghost.erased (BD.lbignum t (v k.AM.bn.BN.len)))
+  (mu:limb t{SM.bn_mont_pre n mu}) : BE.concrete_ops t k.AM.bn.BN.len k.AM.bn.BN.len =
+{
+  BE.to = mk_to_nat_mont_ll_comm_monoid t k.AM.bn.BN.len n mu;
+  BE.lmul = bn_almost_mont_mul k n mu;
+  BE.lsqr = bn_almost_mont_sqr k n mu;
+}
+
+///////////////////////////////////////////////////////////////////////
+
+noextract
+let bn_exp_almost_mont_pre
+  (#t:limb_t)
+  (#len:SN.bn_len t)
+  (n:BD.lbignum t len)
+  (mu:limb t)
+  (r2:BD.lbignum t len)
+  (aM:BD.lbignum t len)
+  (bBits:size_pos)
+  (b:BD.lbignum t (BD.blocks bBits (bits t)))
+ =
+   SM.bn_mont_pre n mu /\
+   BD.bn_v r2 == pow2 (2 * bits t * len) % BD.bn_v n /\
+   BD.bn_v b < pow2 bBits /\
+   BD.bn_v aM < BD.bn_v n
+
+
+inline_for_extraction noextract
+let bn_exp_almost_mont_st (t:limb_t) (len:BN.meta_len t) =
+    n:lbignum t len
+  -> mu:limb t
+  -> r2:lbignum t len
+  -> aM:lbignum t len
+  -> bBits:size_t{v bBits > 0}
+  -> b:lbignum t (blocks bBits (size (bits t)))
+  -> resM:lbignum t len ->
+  Stack unit
+  (requires fun h ->
+    live h n /\ live h aM /\ live h b /\ live h resM /\ live h r2 /\
+    disjoint resM aM /\ disjoint resM b /\ disjoint resM n /\ disjoint n aM /\
+    disjoint resM r2 /\ disjoint aM r2 /\ disjoint n r2 /\ disjoint aM b /\
+
+    bn_exp_almost_mont_pre (as_seq h n) mu (as_seq h r2) (as_seq h aM) (v bBits) (as_seq h b))
+  (ensures  fun h0 _ h1 -> modifies (loc aM |+| loc resM) h0 h1 /\
+   (let k1 = E.mk_nat_mont_ll_comm_monoid (bits t) (v len) (bn_v h0 n) (v mu) in
+    bn_v h1 resM % bn_v h0 n == LE.pow k1 (bn_v h0 aM) (bn_v h0 b)))
+
+
+// This function is *NOT* constant-time on the exponent b.
+inline_for_extraction noextract
+val bn_exp_almost_mont_bm_vartime: #t:limb_t -> k:AM.almost_mont t -> bn_exp_almost_mont_st t k.AM.bn.BN.len
+let bn_exp_almost_mont_bm_vartime #t k n mu r2 aM bBits b resM =
+  [@inline_let] let len = k.AM.bn.BN.len in
+  let h0 = ST.get () in
+  let k1 = Ghost.hide (E.mk_nat_mont_ll_comm_monoid (bits t) (v len) (bn_v h0 n) (v mu)) in
+
+  let bLen = blocks bBits (size (bits t)) in
+  bn_almost_mont_one k n mu r2 resM;
+  BD.bn_eval_bound (as_seq h0 aM) (v len);
+  BE.lexp_rl_vartime len len (mk_bn_almost_mont_concrete_ops t k (as_seq h0 n) mu) n aM bLen bBits b resM;
+  LE.exp_rl_lemma k1 (bn_v h0 aM % bn_v h0 n) (v bBits) (bn_v h0 b);
+  E.pow_nat_mont_ll_mod_base (bits t) (v len) (bn_v h0 n) (v mu) (bn_v h0 aM) (bn_v h0 b)
+
+
+// This function is constant-time on the exponent b.
+inline_for_extraction noextract
+val bn_exp_almost_mont_bm_consttime: #t:limb_t -> k:AM.almost_mont t -> bn_exp_almost_mont_st t k.AM.bn.BN.len
+let bn_exp_almost_mont_bm_consttime #t k n mu r2 aM bBits b resM =
+  [@inline_let] let len = k.AM.bn.BN.len in
+  let h0 = ST.get () in
+  let k1 = Ghost.hide (E.mk_nat_mont_ll_comm_monoid (bits t) (v len) (bn_v h0 n) (v mu)) in
+
+  let bLen = blocks bBits (size (bits t)) in
+  bn_almost_mont_one k n mu r2 resM;
+  BE.lexp_mont_ladder_swap_consttime len len (mk_bn_almost_mont_concrete_ops t k (as_seq h0 n) mu) n aM bLen bBits b resM;
+  LE.exp_mont_ladder_swap_lemma k1 (bn_v h0 aM % bn_v h0 n) (v bBits) (bn_v h0 b);
+  LE.exp_mont_ladder_lemma k1 (bn_v h0 aM % bn_v h0 n) (v bBits) (bn_v h0 b);
+  E.pow_nat_mont_ll_mod_base (bits t) (v len) (bn_v h0 n) (v mu) (bn_v h0 aM) (bn_v h0 b)
+
+
+// This function is *NOT* constant-time on the exponent b.
+inline_for_extraction noextract
+val bn_exp_almost_mont_fw_vartime:
+    #t:limb_t
+  -> k:AM.almost_mont t
+  -> l:size_t{0 < v l /\ v l < bits U32 /\ pow2 (v l) * v k.AM.bn.BN.len <= max_size_t} ->
+  bn_exp_almost_mont_st t k.AM.bn.BN.len
+
+let bn_exp_almost_mont_fw_vartime #t k l n mu r2 aM bBits b resM =
+  [@inline_let] let len = k.AM.bn.BN.len in
+  let h0 = ST.get () in
+  let k1 = Ghost.hide (E.mk_nat_mont_ll_comm_monoid (bits t) (v len) (bn_v h0 n) (v mu)) in
+
+  let bLen = blocks bBits (size (bits t)) in
+  bn_almost_mont_one k n mu r2 resM;
+  BE.lexp_fw_vartime len len (mk_bn_almost_mont_concrete_ops t k (as_seq h0 n) mu) n aM bLen bBits b resM l;
+  LE.exp_fw_lemma k1 (bn_v h0 aM % bn_v h0 n) (v bBits) (bn_v h0 b) (v l);
+  E.pow_nat_mont_ll_mod_base (bits t) (v len) (bn_v h0 n) (v mu) (bn_v h0 aM) (bn_v h0 b)
+
+
+// This function is constant-time on the exponent b.
+inline_for_extraction noextract
+val bn_exp_almost_mont_fw_consttime:
+    #t:limb_t
+  -> k:AM.almost_mont t
+  -> l:size_t{0 < v l /\ v l < bits U32 /\ pow2 (v l) * v k.AM.bn.BN.len <= max_size_t} ->
+  bn_exp_almost_mont_st t k.AM.bn.BN.len
+
+let bn_exp_almost_mont_fw_consttime #t k l n mu r2 aM bBits b resM =
+  [@inline_let] let len = k.AM.bn.BN.len in
+  let h0 = ST.get () in
+  let k1 = Ghost.hide (E.mk_nat_mont_ll_comm_monoid (bits t) (v len) (bn_v h0 n) (v mu)) in
+
+  let bLen = blocks bBits (size (bits t)) in
+  bn_almost_mont_one k n mu r2 resM;
+  BE.lexp_fw_consttime len len (mk_bn_almost_mont_concrete_ops t k (as_seq h0 n) mu) n aM bLen bBits b resM l;
+  LE.exp_fw_lemma k1 (bn_v h0 aM % bn_v h0 n) (v bBits) (bn_v h0 b) (v l);
+  E.pow_nat_mont_ll_mod_base (bits t) (v len) (bn_v h0 n) (v mu) (bn_v h0 aM) (bn_v h0 b)
+
+///////////////////////////////////////////////
+
+// This function is *NOT* constant-time on the exponent b.
+inline_for_extraction noextract
+val bn_exp_almost_mont_vartime: #t:limb_t -> k:AM.almost_mont t -> bn_exp_almost_mont_st t k.AM.bn.BN.len
+let bn_exp_almost_mont_vartime #t k n mu r2 aM bBits b resM =
+  if bBits <. size ME.bn_exp_mont_vartime_threshold then
+    bn_exp_almost_mont_bm_vartime k n mu r2 aM bBits b resM
+  else
+    bn_exp_almost_mont_fw_vartime k 4ul n mu r2 aM bBits b resM
+
+
+// This function is constant-time on the exponent b.
+inline_for_extraction noextract
+val bn_exp_almost_mont_consttime: #t:limb_t -> k:AM.almost_mont t -> bn_exp_almost_mont_st t k.AM.bn.BN.len
+let bn_exp_almost_mont_consttime #t k n mu r2 aM bBits b resM =
+  if bBits <. size ME.bn_exp_mont_consttime_threshold then
+    bn_exp_almost_mont_bm_consttime k n mu r2 aM bBits b resM
+  else
+    bn_exp_almost_mont_fw_consttime k 4ul n mu r2 aM bBits b resM
